dev2020/dsubsup_cc/cc_meta.v
@@ -6,9 +6,34 @@ Require Import Coq.Lists.List.
 Import ListNotations.
 
 Require Import languages.
-(* make ⋆ and ◻ available *)
 Import CC.Notations.
 Open Scope cc_scope.
 
+Import CC.
+
+Lemma open_identity: forall b b' f u t,
+    closed b f t ->
+    b' >= b ->
+    (open_rec b' u t) = t.
+Proof.
+Admitted.
+
+Lemma subst_identity: forall b f f' u t,
+    closed b f t ->
+    f' >= f ->
+    (subst f u t) = t.
+Proof.
+Admitted.
+
+(* TODO: prove that (T^e) = (T^x){e/x} *)
+Lemma open_subst: forall b b' f u t,
+    closed b f t ->
+    (open_rec b' u t) = (subst f u (open_rec b' (tvar (varF f)) t)).
+Proof.
+Admitted.
 
 (* TODO prove strong normalization *)
+Theorem full_total_safety : strong_normalization.
+Proof.
+  unfold strong_normalization.
+Admitted.
